theories/examples/awkward_example_adequacy.v
@@ -1,12 +1,13 @@
-From iris.algebra Require Import frac.
+From iris.algebra Require Import auth agree excl gmap frac.
 From iris.proofmode Require Import tactics.
 From iris.base_logic Require Import invariants.
+From iris.program_logic Require Import adequacy.
 Require Import Eqdep_dec.
 From cap_machine Require Import
-     rules logrel fundamental region_invariants
+     rules logrel fundamental region_invariants sts
      region_invariants_revocation region_invariants_static.
 From cap_machine.examples Require Import
-     region_macros malloc awkward_example awkward_example_preamble.
+     stack_macros malloc awkward_example awkward_example_preamble.
 
 Instance DisjointList_list_Addr : DisjointList (list Addr).
 Proof. exact (@disjoint_list_default _ _ app []). Defined.
@@ -14,23 +15,55 @@ Proof. exact (@disjoint_list_default _ _ app []). Defined.
 Class memory_layout := {
   (* awkward example: preamble & body *)
   awk_region_start : Addr;
+  awk_preamble_start : Addr;
+  awk_body_start : Addr;
   awk_region_end : Addr;
 
-  awk_region_size :
-    (awk_region_start
-     + (1 (* pointer to the linking table *)
-        + awkward_preamble_instrs_length (* preamble instructions *)
-        + awkward_instrs_length (* closure body instructions *))
-    )%a
+  (* pointer to the linking table, at the beginning of the region *)
+  awk_linking_ptr_size :
+    (awk_region_start + 1)%a = Some awk_preamble_start;
+
+  (* preamble code, that allocates the closure *)
+  awk_preamble_size :
+    (awk_preamble_start + awkward_preamble_instrs_length)%a
+    = Some awk_body_start;
+
+  (* code of the body, wrapped in the closure allocated by the preamble *)
+  awk_body_size :
+    (awk_body_start + awkward_instrs_length)%a
     = Some awk_region_end;
 
+  (* stack *)
+  stack_start : Addr;
+  stack_end : Addr;
+
+  (* adversary code *)
+  adv_start : Addr;
+  adv_end : Addr;
+
   (* malloc routine *)
+  (* TODO: more general malloc spec *)
+(*
   malloc_start : Addr;
   malloc_end : Addr;
+
+  malloc_size :
+    (malloc_start + length malloc_subroutine)%a
+    = Some malloc_end; *)
+  malloc_size :
+    (b_m + length malloc_subroutine)%a
+    = Some e_m;
 
   (* fail routine *)
   fail_start : Addr;
   fail_end : Addr;
+
+  fail_size :
+    (fail_start
+     + (length assert_fail_instrs (* code of the subroutine *)
+        + 1 (* pointer to the flag *))
+    )%a
+    = Some fail_end;
 
   (* link table *)
   link_table_start : Addr;
@@ -39,28 +72,491 @@ Class memory_layout := {
   link_table_size :
     (link_table_start + 2)%a = Some link_table_end;
 
+  (* failure flag *)
+  fail_flag : Addr;
+  fail_flag_next : Addr;
+  fail_flag_size :
+    (fail_flag + 1)%a = Some fail_flag_next;
+
   (* disjointness of all the regions above *)
   regions_disjoint :
-    ## [region_addrs awk_region_start awk_region_end;
-        region_addrs malloc_start malloc_end;
+    ## [
+        [fail_flag];
+        region_addrs link_table_start link_table_end;
         region_addrs fail_start fail_end;
-        region_addrs link_table_start link_table_end];
+        region_addrs b_m e_m;
+        region_addrs adv_start adv_end;
+        region_addrs stack_start stack_end;
+        region_addrs awk_body_start awk_region_end;
+        region_addrs awk_preamble_start awk_body_start;
+        [awk_region_start]
+       ];
 }.
 
 Definition mkregion (r_start r_end: Addr) (contents: list Word): gmap Addr Word :=
   list_to_map (zip (region_addrs r_start r_end) contents).
 
-Definition initial_memory_spec `{memory_layout} (m m_adv: gmap Addr Word) :=
-  m =   mkregion awk_region_start awk_region_end
-          ((* pointer to the linking table *)
-           [inr (RW, Global, link_table_start, link_table_end, link_table_start)] ++
+Definition offset_to_awkward `{memory_layout} : Z :=
+  (* in this setup, the body of the awkward examples comes just after the code
+     of the preamble *)
+  (awkward_preamble_instrs_length - awkward_preamble_move_offset)%Z.
+
+(* FIXME: the link table permission could be restricted to RO *)
+Definition is_initial_memory `{memory_layout} (m: gmap Addr Word) :=
+  ∃ (adv_val stack_val: list Word),
+  m =   (* pointer to the linking table *)
+        list_to_map [(awk_region_start,
+                      inr (RW, Global, link_table_start, link_table_end, link_table_start))]
+      ∪ mkregion awk_preamble_start awk_body_start
            (* preamble: code that creates the awkward example closure *)
-           awkward_preamble_instrs 0%Z (* offset to malloc in linking table *)
-             0%Z (* ?? *) ++
+          (awkward_preamble_instrs 0%Z (* offset to malloc in linking table *)
+             offset_to_awkward (* offset to the body of the example *))
+      ∪ mkregion awk_body_start awk_region_end
            (* body of the awkward example, that will be encapsulated in the closure
               created by the preamble *)
-           awkward_instrs r_t0 (* ?? *) 0%Z (* ?? *))
-      ∪ mkregion malloc_start malloc_end malloc_subroutine
-      ∪ m_adv
+          (awkward_instrs 1%Z (* offset to fail in the linking table *)
+             r_adv (* register used to call to arbitrary code *))
+      ∪ mkregion stack_start stack_end
+          (* initial content of the stack: can be anything *)
+          stack_val
+      ∪ mkregion adv_start adv_end
+          (* adversarial code: any code or data, but no capabilities (see condition below) *)
+          adv_val
+      ∪ mkregion b_m e_m
+          (* code for the malloc subroutine *)
+          malloc_subroutine
+      ∪ mkregion fail_start fail_end
+          ((* code for the failure subroutine *)
+            assert_fail_instrs ++
+           (* pointer to the "failure" flag, set to 1 by the routine *)
+           [inr (RW, Global, fail_flag, fail_flag_next, fail_flag)])
+      ∪ mkregion link_table_start link_table_end
+          (* link table, with pointers to the malloc and failure subroutines *)
+          [inr (E, Global, b_m, e_m, a_m);
+           inr (E, Global, fail_start, fail_end, fail_start)]
+      ∪ list_to_map [(fail_flag, inl 0%Z)] (* failure flag, initially set to 0 *)
   ∧
-  (∀ a w, m_adv !! a = Some w → is_cap w = false).
+  (* the adversarial region in memory must only contain instructions, no
+     capabilities (it can thus only access capabilities the awkward preamble
+     passes it through the registers) *)
+  Forall (λ w, is_cap w = false) adv_val
+  ∧
+  (adv_start + length adv_val)%a = Some adv_end
+  ∧
+  (stack_start + length stack_val)%a = Some stack_end.
+
+Definition is_initial_registers `{memory_layout} (reg: gmap RegName Word) :=
+  reg !! PC = Some (inr (RX, Global, awk_region_start, awk_region_end, awk_preamble_start)) ∧
+  reg !! r_stk = Some (inr ((*TODO: U*)RWLX, Local, stack_start, stack_end, stack_start)) ∧
+  reg !! r_t0 = Some (inr (RWX, Global, adv_start, adv_end, adv_start)) ∧
+  (∀ (r: RegName), r ∉ ({[ PC; r_stk; r_t0 ]} : gset RegName) →
+    ∃ (w:Word), reg !! r = Some w ∧ is_cap w = false).
+
+Lemma initial_registers_full_map `{memory_layout} reg :
+  is_initial_registers reg →
+  (∀ r, is_Some (reg !! r)).
+Proof.
+  intros (HPC & Hstk & H0 & Hothers) r.
+  destruct (decide (r = PC)) as [->|]. by eauto.
+  destruct (decide (r = r_stk)) as [->|]. by eauto.
+  destruct (decide (r = r_t0)) as [->|]. by eauto.
+  destruct (Hothers r) as (w & ? & ?); [| eauto]. set_solver.
+Qed.
+
+(* TODO: move elsewhere *)
+Section WorldUpdates.
+  Context {Σ:gFunctors} {memg:memG Σ} {regg:regG Σ}
+          {stsg : STSG Addr region_type Σ} {heapg : heapG Σ}
+          `{MonRef: MonRefG (leibnizO _) CapR_rtc Σ}.
+
+  Notation STS := (leibnizO (STS_states * STS_rels)).
+  Notation STS_STD := (leibnizO (STS_std_states Addr region_type)).
+  Notation WORLD := (prodO STS_STD STS).
+  Implicit Types W : WORLD.
+
+  Lemma extend_region_perm_sepL2 E W l1 l2 p φ `{∀ Wv, Persistent (φ Wv)}:
+     p ≠ O →
+     Forall (λ k, std W !! k = None) l1 →
+     (sts_full_world W -∗ region W -∗
+     ([∗ list] k;v ∈ l1;l2, k ↦ₐ[p] v ∗ φ (W, v) ∗ future_priv_mono φ v)
+
+     ={E}=∗
+
+     region (std_update_multiple W l1 Permanent)
+     ∗ ([∗ list] k ∈ l1, rel k p φ)
+     ∗ sts_full_world (std_update_multiple W l1 Permanent))%I.
+  Proof.
+    revert l2. induction l1.
+    { cbn. intros. iIntros "? ? ?". iFrame. eauto. }
+    { intros * ? [? ?]%Forall_cons_1. iIntros "Hsts Hr Hl".
+      iDestruct (big_sepL2_length with "Hl") as %Hlen.
+      iDestruct (NoDup_of_sepL2_exclusive with "[] Hl") as %[Hal1 ND]%NoDup_cons.
+      { iIntros (? ? ?) "(H1 & ? & ?) (H2 & ? & ?)".
+        iApply (cap_duplicate_false with "[$H1 $H2]"). auto. }
+      destruct l2; [ by inversion Hlen |].
+      iDestruct (big_sepL2_cons with "Hl") as "[(Ha & Hφ & #Hf) Hl]".
+      iMod (IHl1 with "Hsts Hr Hl") as "(Hr & ? & Hsts)"; auto.
+      iDestruct (extend_region_perm with "Hf Hsts Hr Ha [Hφ]") as ">(? & ? & ?)"; auto.
+      { rewrite -std_update_multiple_not_in_sta; auto.
+        rewrite not_elem_of_dom //. }
+      { iApply ("Hf" with "[] Hφ"). iPureIntro.
+        apply related_sts_pub_priv_world, related_sts_pub_update_multiple.
+        eapply Forall_impl; eauto.
+        intros. by rewrite not_elem_of_dom. }
+      iModIntro. cbn. iFrame. }
+  Qed.
+
+End WorldUpdates.
+
+Section Adequacy.
+  Context (Σ: gFunctors).
+  Context {inv_preg: invPreG Σ}.
+  Context {mem_preg: gen_heapPreG Addr Word Σ}.
+  Context {reg_preg: gen_heapPreG RegName Word Σ}.
+  Context {MonRef: @MonRefG (leibnizO _) CapR_rtc Σ}.
+  Context {na_invg: na_invG Σ}.
+  Context {sts_preg: STS_preG Addr region_type Σ}.
+  Context {heappreg: heapPreG Σ}.
+
+  Notation STS := (leibnizO (STS_states * STS_rels)).
+  Notation STS_STD := (leibnizO (STS_std_states Addr region_type)).
+  Notation WORLD := (prodO STS_STD STS).
+
+  Lemma dom_mkregion_incl a e l:
+    dom (gset Addr) (mkregion a e l) ⊆ list_to_set (region_addrs a e).
+  Proof.
+    rewrite /mkregion. generalize (region_addrs a e). induction l.
+    { intros. rewrite zip_with_nil_r /=. rewrite dom_empty_L. apply empty_subseteq. }
+    { intros ll. destruct ll as [| x ll].
+      - cbn. rewrite dom_empty_L. done.
+      - cbn [list_to_set zip zip_with list_to_map foldr fst snd]. rewrite dom_insert_L.
+        set_solver. }
+  Qed.
+
+  Lemma disjoint_mono_l A C `{ElemOf A C} (X Y Z: C) : X ⊆ Y → Y ## Z → X ## Z.
+  Proof. intros * HXY. rewrite !elem_of_disjoint. eauto. Qed.
+
+  Lemma disjoint_mono_r A C `{ElemOf A C} (X Y Z: C) : X ⊆ Y → Z ## Y → Z ## X.
+  Proof. intros * HXY. rewrite !elem_of_disjoint. eauto. Qed.
+
+  Lemma dom_list_to_map_singleton (x:Addr) (y:Word):
+    dom (gset Addr) (list_to_map [(x, y)] : gmap Addr Word) = list_to_set [x].
+  Proof. rewrite dom_insert_L /= dom_empty_L. set_solver. Qed.
+
+  Lemma list_to_set_disj (l1 l2: list Addr) : l1 ## l2 → (list_to_set l1: gset Addr) ## list_to_set l2.
+  Proof.
+    intros * HH. rewrite elem_of_disjoint. intros x.
+    rewrite !elem_of_list_to_set. rewrite elem_of_disjoint in HH |- *. eauto.
+  Qed.
+
+  Ltac disjoint_map_to_list :=
+    rewrite (@map_disjoint_dom _ _ (gset Addr)) ?dom_union_L;
+    eapply disjoint_mono_l;
+    repeat lazymatch goal with
+           | |- _ ∪ _ ⊆ _ =>
+             etransitivity; [ eapply union_mono_l; apply dom_mkregion_incl
+                            | eapply union_mono_r ]
+           | |- _ ⊆ _ => first [ apply dom_mkregion_incl
+                               | by rewrite dom_list_to_map_singleton ]
+           end;
+    try match goal with |- _ ## dom _ (mkregion _ _ _) =>
+      eapply disjoint_mono_r; [ apply dom_mkregion_incl |] end;
+    rewrite -?list_to_set_app_L ?dom_list_to_map_singleton;
+    apply list_to_set_disj.
+
+  Lemma region_addrs_cons a e :
+    (a < e)%a →
+    region_addrs a e = a :: region_addrs (^(a+1))%a e.
+  Proof.
+    intros. rewrite (region_addrs_decomposition a a). 2: solve_addr.
+    rewrite /region_addrs region_size_0 //. solve_addr.
+  Qed.
+
+  Lemma elem_of_region_addrs (a b e: Addr):
+    a ∈ region_addrs b e ↔ (b <= a)%a ∧ (a < e)%a.
+  Proof.
+    rewrite /region_addrs /region_size.
+    set n := Z.to_nat (e - b). have: (n = Z.to_nat (e - b)) by reflexivity.
+    clearbody n. revert n a b e. induction n.
+    { intros. cbn. rewrite elem_of_nil. solve_addr. }
+    { intros. cbn. rewrite elem_of_cons (IHn a _ e). 2: solve_addr.
+      split. intros [ -> | ]; solve_addr. intros [Hba ?].
+      apply Zle_lt_or_eq in Hba. destruct Hba; [| subst]. solve_addr.
+      assert (b = a) by solve_addr. subst. solve_addr. }
+  Qed.
+
+  Lemma contiguous_between_region_addrs a e :
+    (a <= e) %a → contiguous_between (region_addrs a e) a e.
+  Proof. intros; by apply contiguous_between_of_region_addrs. Qed.
+
+  Lemma mkregion_sepM_to_sepL2 (a e: Addr) l (φ: Addr → Word → iProp Σ) :
+    (a + length l)%a = Some e →
+    ([∗ map] k↦v ∈ mkregion a e l, φ k v) -∗ ([∗ list] k;v ∈ (region_addrs a e); l, φ k v).
+  Proof.
+    rewrite /mkregion. revert a e. induction l as [| x l].
+    { cbn. intros. rewrite zip_with_nil_r /=. assert (a = e) as -> by solve_addr.
+      rewrite /region_addrs region_size_0. 2: solve_addr. cbn. eauto. }
+    { cbn. intros a e Hlen. rewrite region_addrs_cons. 2: solve_addr.
+      cbn. iIntros "H". iDestruct (big_sepM_insert with "H") as "[? H]".
+      { rewrite -not_elem_of_list_to_map /=.
+        intros [ [? ?] [-> [? ?]%elem_of_zip_l%elem_of_region_addrs] ]%elem_of_list_fmap.
+        solve_addr. }
+      iFrame. iApply (IHl with "H"). solve_addr. }
+  Qed.
+
+  (* TODO: move to iris? *)
+  Lemma big_sepL2_bupd
+     : ∀ (PROP : bi) (H : BiBUpd PROP) (A B : Type) (Φ : A → B → PROP) (l1 : list A) (l2: list B),
+         ([∗ list] k;x ∈ l1;l2, |==> Φ k x) -∗ |==> [∗ list] k;x ∈ l1;l2, Φ k x.
+  Proof.
+    intros. revert l2. induction l1 as [| x l1].
+    { intros. iIntros "H".
+      iDestruct (big_sepL2_length with "H") as %Hlen. cbn in Hlen.
+      destruct l2; [| by inversion Hlen]. cbn. eauto. }
+    { intros. iIntros "H".
+      iDestruct (big_sepL2_length with "H") as %Hlen. cbn in Hlen.
+      destruct l2; [by inversion Hlen |]. cbn. iDestruct "H" as "[>? H]".
+      iDestruct (IHl1 with "H") as ">?". iModIntro. iFrame. }
+  Qed.
+
+  Lemma MonRefAlloc_sepL2 `{memG Σ} (p:Perm) (l1: list Addr) (l2: list Word) :
+    ([∗ list] k;v ∈ l1;l2, k ↦ₐ v) ==∗ ([∗ list] k;v ∈ l1;l2, k ↦ₐ[p] v).
+  Proof.
+    iIntros "H".
+    iDestruct (big_sepL2_mono with "H") as "H".
+    { intros. apply MonRefAlloc. }
+    SearchAbout "bupd" "sepL".
+    iDestruct (big_sepL2_bupd with "H") as "H". eauto.
+  Qed.
+
+  Lemma mkregion_prepare `{memG Σ} p (a e: Addr) l :
+    (a + length l)%a = Some e →
+    ([∗ map] k↦v ∈ mkregion a e l, k ↦ₐ v) ==∗ ([∗ list] k;v ∈ (region_addrs a e); l, k ↦ₐ[p] v).
+  Proof.
+    iIntros (?) "H". iDestruct (mkregion_sepM_to_sepL2 with "H") as "H"; auto.
+    iMod (MonRefAlloc_sepL2 with "H"). eauto.
+  Qed.
+
+  Definition flagN : namespace := nroot .@ "awk" .@ "fail_flag".
+
+  Lemma awkward_example_adequacy `{memory_layout} (m m': Mem) (reg reg': Reg) (es: list cap_lang.expr):
+    is_initial_memory m →
+    is_initial_registers reg →
+    rtc erased_step ([Seq (Instr Executable)], (reg, m)) (es, (reg', m')) →
+    m' !! fail_flag = Some (inl 0%Z).
+  Proof.
+    intros Hm Hreg Hstep.
+    pose proof (@wp_invariance Σ cap_lang _ NotStuck) as WPI. cbn in WPI.
+    pose (fun (c: ExecConf) => c.2 !! fail_flag = Some (inl 0%Z)) as state_is_good.
+    specialize (WPI (Seq (Instr Executable)) (reg, m) es (reg', m') (state_is_good (reg', m'))).
+    eapply WPI. 2: assumption. intros Hinv κs. clear WPI.
+
+    destruct Hm as (adv_val & stack_val & Hm & Hadv_val & adv_size & stack_size).
+    iMod (gen_heap_init (∅:Mem)) as (mem_heapg) "Hmem_ctx".
+    iMod (gen_heap_init (∅:Reg)) as (reg_heapg) "Hreg_ctx".
+    unshelve iMod gen_sts_init as (stsg) "Hsts"; eauto. (*XX*)
+    set W0 := ((∅, (∅, ∅)) : WORLD).
+    iMod heap_init as (heapg) "HRELS".
+    iMod (@na_alloc Σ na_invg) as (logrel_nais) "Hna".
+
+    pose memg := MemG Σ Hinv mem_heapg.
+    pose regg := RegG Σ Hinv reg_heapg.
+    pose logrel_na_invs := Build_logrel_na_invs _ na_invg logrel_nais.
+
+    pose proof (
+      @awkward_preamble_spec Σ memg regg stsg heapg MonRef logrel_na_invs
+    ) as Spec.
+
+    iMod (gen_heap_alloc_gen _ reg with "Hreg_ctx") as "(Hreg_ctx & Hreg & _)".
+      by apply map_disjoint_empty_r. rewrite right_id_L.
+    iMod (gen_heap_alloc_gen _ m with "Hmem_ctx") as "(Hmem_ctx & Hmem & _)".
+      by apply map_disjoint_empty_r. rewrite right_id_L.
+
+    (* Extract points-to for the various regions in memory *)
+
+    pose proof regions_disjoint as Hdisjoint.
+    rewrite {2}Hm.
+    rewrite disjoint_list_cons in Hdisjoint |- *. intros (Hdisj_fail_flag & Hdisjoint).
+    iDestruct (big_sepM_union with "Hmem") as "[Hmem Hfail_flag]".
+    { disjoint_map_to_list. set_solver +Hdisj_fail_flag. }
+    iDestruct (big_sepM_insert with "Hfail_flag") as "[Hfail_flag _]".
+      by apply lookup_empty. cbn [fst snd].
+    rewrite disjoint_list_cons in Hdisjoint |- *. intros (Hdisj_link_table & Hdisjoint).
+    iDestruct (big_sepM_union with "Hmem") as "[Hmem Hlink_table]".
+    { disjoint_map_to_list. set_solver +Hdisj_link_table. }
+    rewrite disjoint_list_cons in Hdisjoint |- *. intros (Hdisj_fail & Hdisjoint).
+    iDestruct (big_sepM_union with "Hmem") as "[Hmem Hfail]".
+    { disjoint_map_to_list. set_solver +Hdisj_fail. }
+    rewrite disjoint_list_cons in Hdisjoint |- *. intros (Hdisj_malloc & Hdisjoint).
+    iDestruct (big_sepM_union with "Hmem") as "[Hmem Hmalloc]".
+    { disjoint_map_to_list. set_solver +Hdisj_malloc. }
+    rewrite disjoint_list_cons in Hdisjoint |- *. intros (Hdisj_adv & Hdisjoint).
+    iDestruct (big_sepM_union with "Hmem") as "[Hmem Hadv]".
+    { disjoint_map_to_list. set_solver +Hdisj_adv. }
+    rewrite disjoint_list_cons in Hdisjoint |- *. intros (Hdisj_stack & Hdisjoint).
+    iDestruct (big_sepM_union with "Hmem") as "[Hmem Hstack]".
+    { disjoint_map_to_list. set_solver +Hdisj_stack. }
+    rewrite disjoint_list_cons in Hdisjoint |- *. intros (Hdisj_awk_body & Hdisjoint).
+    iDestruct (big_sepM_union with "Hmem") as "[Hmem Hawk_body]".
+    { disjoint_map_to_list. set_solver +Hdisj_awk_body. }
+    rewrite disjoint_list_cons in Hdisjoint |- *. intros (Hdisj_awk_preamble & _).
+    iDestruct (big_sepM_union with "Hmem") as "[Hawk_link Hawk_preamble]".
+    { disjoint_map_to_list. set_solver +Hdisj_awk_preamble. }
+    iDestruct (big_sepM_insert with "Hawk_link") as "[Hawk_link _]". by apply lookup_empty.
+    cbn [fst snd].
+    clear Hdisj_fail_flag Hdisj_link_table Hdisj_fail Hdisj_malloc Hdisj_adv Hdisj_stack
+      Hdisj_awk_body Hdisj_awk_preamble.
+
+    (* Massage points-to into sepL2s with permission-pointsto *)
+
+    iDestruct (mkregion_prepare RW with "Hlink_table") as ">Hlink_table". by apply link_table_size.
+    iDestruct (mkregion_prepare RW with "Hfail") as ">Hfail". by apply fail_size.
+    iDestruct (mkregion_prepare p_m with "Hmalloc") as ">Hmalloc". by apply malloc_size.
+    iDestruct (mkregion_prepare RWX with "Hadv") as ">Hadv". by apply adv_size.
+    iDestruct (mkregion_prepare RWLX with "Hstack") as ">Hstack". by apply stack_size.
+    iDestruct (mkregion_prepare RWX with "Hawk_preamble") as ">Hawk_preamble".
+      by apply awk_preamble_size.
+    iDestruct (mkregion_prepare RWX with "Hawk_body") as ">Hawk_body". by apply awk_body_size.
+    iMod (MonRefAlloc _ _ RWX (* FIXME?? *) with "Hawk_link") as "Hawk_link".
+    rewrite -/(awkward_example _ _ _ _) -/(awkward_preamble _ _ _ _).
+    rewrite -/(region_mapsto b_m e_m p_m malloc_subroutine).
+
+    (* Split the link table *)
+
+    rewrite (region_addrs_cons link_table_start link_table_end).
+    2: { generalize link_table_size; clear; solve_addr. }
+    set link_entry_fail := ^(link_table_start + 1)%a.
+    rewrite (region_addrs_cons link_entry_fail link_table_end).
+    2: { generalize link_table_size; clear. subst link_entry_fail.
+         generalize link_table_start link_table_end. solve_addr. }
+    rewrite (_: ^(link_entry_fail + 1)%a = link_table_end).
+    2: { generalize link_table_size; clear. subst link_entry_fail.
+         generalize link_table_start link_table_end. solve_addr. }
+    iDestruct (big_sepL2_cons with "Hlink_table") as "[Hlink1 Hlink_table]".
+    iDestruct (big_sepL2_cons with "Hlink_table") as "[Hlink2 _]".
+
+    (* Allocate relevant invariants *)
+
+    iMod (inv_alloc flagN ⊤ (fail_flag ↦ₐ inl 0%Z) with "Hfail_flag")%I as "#Hinv_fail_flag".
+    iMod (inv_alloc malloc_γ ⊤ with "Hmalloc") as "#Hinv_malloc".
+
+    (* Allocate a permanent region for the adversary code *)
+
+    iAssert (region W0) with "[HRELS]" as "Hr".
+    { rewrite region_eq /region_def. iExists ∅, ∅. iFrame.
+      rewrite /= !dom_empty_L //. repeat iSplit; eauto.
+      rewrite /region_map_def. by rewrite big_sepM_empty. }
+
+    iMod (extend_region_perm_sepL2 _ _ _ _ RWX (λ Wv, interp Wv.1 Wv.2)
+            with "Hsts Hr [Hadv]") as "(Hr & Hadv & Hsts)".
+    3: { iApply (big_sepL2_mono with "Hadv").
+         intros k v1 v2 Hv1 Hv2. cbn. iIntros. iFrame.
+         pose proof (Forall_lookup_1 _ _ _ _ Hadv_val Hv2) as Hncap.
+         destruct v2; [| by inversion Hncap].
+         rewrite fixpoint_interp1_eq /=. iSplit; eauto.
+         unfold future_priv_mono. iModIntro. iIntros.
+         rewrite !fixpoint_interp1_eq //=. }
+    done.
+    { rewrite Forall_lookup. intros. cbn.
+      eapply (@lookup_empty _ (gmap Addr)); typeclasses eauto. }
+    iDestruct "Hadv" as "#Hadv".
+
+    set W1 := (std_update_multiple W0 (region_addrs adv_start adv_end) Permanent).
+
+    (* Apply the spec, obtain that the PC is in the expression relation *)
+
+    iAssert (((interp_expr interp reg) W1) (inr (RX, Global, awk_region_start, awk_region_end, awk_preamble_start)))
+      with "[Hawk_preamble Hawk_body Hinv_malloc Hawk_link Hlink1 Hlink2]" as "HE".
+    { assert (isCorrectPC_range RX Global awk_region_start awk_region_end
+                                awk_preamble_start awk_body_start).
+      { intros a [Ha1 Ha2]. constructor; auto.
+        generalize awk_linking_ptr_size awk_preamble_size awk_body_size. revert Ha1 Ha2. clear.
+        unfold awkward_instrs_length, awkward_preamble_instrs_length. solve_addr. }
+      set awk_preamble_move_addr := ^(awk_preamble_start + awkward_preamble_move_offset)%a.
+      assert ((awk_preamble_start + awkward_preamble_move_offset)%a = Some awk_preamble_move_addr).
+      { clear. subst awk_preamble_move_addr.
+        generalize awk_preamble_size.
+        unfold awkward_preamble_instrs_length, awkward_preamble_move_offset.
+        generalize awk_preamble_start awk_body_start. solve_addr. }
+      assert (awk_preamble_move_addr + offset_to_awkward = Some awk_body_start)%a.
+      { generalize awk_preamble_size.
+        unfold awk_preamble_move_addr, offset_to_awkward, awkward_preamble_instrs_length.
+        unfold awkward_preamble_move_offset. clear.
+        generalize awk_preamble_start awk_body_start. solve_addr. }
+      assert (isCorrectPC_range RX Global awk_region_start awk_region_end
+                                awk_body_start awk_region_end).
+      { intros a [Ha1 Ha2]. constructor; auto.
+        generalize awk_linking_ptr_size awk_preamble_size awk_body_size. revert Ha1 Ha2; clear.
+        unfold awkward_instrs_length, awkward_preamble_instrs_length. solve_addr. }
+
+      iApply (Spec with "[$]"); try eassumption.
+      - done.
+      - apply contiguous_between_region_addrs. generalize awk_preamble_size; clear.
+        unfold awkward_preamble_instrs_length. solve_addr.
+      - apply le_addr_withinBounds. clear; solve_addr.
+        generalize link_table_size; clear; solve_addr.
+      - subst link_entry_fail. apply le_addr_withinBounds.
+        generalize link_table_start; clear; solve_addr.
+        generalize link_table_start link_table_end link_table_size. clear; solve_addr.
+      - clear; generalize link_table_start; solve_addr.
+      - clear; subst link_entry_fail;
+        generalize link_table_start link_table_end link_table_size; solve_addr.
+      - apply contiguous_between_region_addrs. generalize awk_body_size; clear.
+        unfold awkward_instrs_length. solve_addr. }
+
+    clear Hm Spec. rewrite /interp_expr /=.
+
+    (* prepare registers *)
+
+    unfold is_initial_registers in Hreg.
+    destruct Hreg as (HPC & Hstk & Hr0 & Hrothers).
+
+    iSpecialize ("HE" with "[Hreg Hr Hsts Hna]").
+    { iFrame. iSplit; cycle 1.
+      { iFrame. rewrite /registers_mapsto. by rewrite insert_id. }
+      { iSplit. iPureIntro; intros; by apply initial_registers_full_map.
+        (* All capabilities in registers are valid! *)
+        iIntros (r HrnPC).
+        (* r0 (return pointer to the adversary) is valid. Prove it using the
+           fundamental theorem. *)
+        destruct (decide (r = r_t0)) as [ -> |].
+        { rewrite /RegLocate Hr0 fixpoint_interp1_eq /=.
+          iExists RWX.
+          iAssert
+            ([∗ list] a ∈ region_addrs adv_start adv_end,
+               read_write_cond a RWX (fixpoint interp1) ∧ ⌜std W1 !! a = Some Permanent⌝)%I
+            as "#Hrwcond".
+          { iApply (big_sepL_mono with "Hadv"). iIntros (k v Hkv). cbn.
+            iIntros "H". rewrite /read_write_cond /=. iFrame. iPureIntro.
+            eapply std_sta_update_multiple_lookup_in_i, elem_of_list_lookup_2; eauto. }
+          iSplitR; auto. iSplit. iApply "Hrwcond". iModIntro.
+          unfold exec_cond. iIntros. iNext. iApply fundamental; auto.
+          iExists RWX. iSplit; auto.
+          iApply (big_sepL_mono with "Hrwcond"). intros. cbn. iIntros "[? %]". iFrame.
+          iPureIntro. eapply region_state_nwl_monotone_nl; eauto. }
+
+        (* Stack *)
+        destruct (decide (r = r_stk)) as [ -> |].
+        { rewrite /RegLocate Hstk fixpoint_interp1_eq /=.
+          admit. (* TODO: true with a URWLX, completely uninitialized stack *) }
+
+        (* Other registers *)
+        rewrite /RegLocate.
+        destruct (Hrothers r) as [rw [Hrw Hncap] ]. set_solver.
+        destruct rw; [| by inversion Hncap].
+        by rewrite Hrw fixpoint_interp1_eq /=. } }
+
+    iDestruct "HE" as "[_ HWP]". unfold interp_conf.
+
+    iModIntro.
+    (* Same as the state_interp of [memG_irisG] in rules_base.v *)
+    iExists (fun σ κs _ => ((gen_heap_ctx σ.1) ∗ (gen_heap_ctx σ.2)))%I.
+    iExists (fun _ => True)%I. cbn. iFrame.
+    iSplitL "HWP". { iApply (wp_wand with "HWP"). eauto. }
+    iIntros "[Hreg' Hmem']". iExists (⊤ ∖ ↑flagN).
+    iInv flagN as ">Hflag" "Hclose".
+    iDestruct (gen_heap_valid with "Hmem' Hflag") as %Hm'_flag.
+    iModIntro. iPureIntro. apply Hm'_flag.
+  Admitted.
+
+End Adequacy.
